case-studies/kathrin/coq/core.v
@@ -76,8 +76,8 @@ Defined.
 Hint Rewrite in_map_iff : FunctorInstances.
 
 (* Declaring the scopes that all our notations will live in *)
-(* Declare Scope fscope. *)
-(* Declare Scope subst_scope. *)
+(* not supported in Coq 8.9 *)
+(* not supported in Coq 8.9 *)
 
 Ltac eta_reduce :=
   repeat match goal with
